stdlib/ptr/output/ptr/proofs/proof_mut_ptr_read.v
@@ -1,0 +1,22 @@
+From caesium Require Import lang notation.
+From refinedrust Require Import typing shims.
+From stdlib.ptr.ptr.generated Require Import generated_code_ptr generated_specs_ptr generated_template_mut_ptr_read.
+
+Set Default Proof Using "Type".
+
+Section proof.
+Context `{RRGS : !refinedrustGS Σ}.
+
+Lemma mut_ptr_read_proof (π : thread_id) :
+  mut_ptr_read_lemma π.
+Proof.
+  mut_ptr_read_prelude.
+
+  repeat liRStep; liShow.
+
+  all: print_remaining_goal.
+  Unshelve. all: sidecond_solver.
+  Unshelve. all: sidecond_hammer.
+  Unshelve. all: print_remaining_sidecond.
+Qed.
+End proof.
